Change behavior of 'decreases *', which can be applied to loops and methods.  Now, loops that may possibly do an infinite number of iterations (that is, loops marked with 'decreases *') and calls to methods marked with 'decreases *' are allowed only in methods that themselves are marked with 'decreases *'.  As before, ghost loops and ghost methods are not allowed to be marked with 'decreases *'.
Previously, 'decreases *' was allowed on a method only if the method was tail recursive;
this is no longer so.  Note, however, that if the method is not tail recursive and engages
in infinite recursion, then it will eventually run out of stack space.

Previously, a 'decreases *' was not inherited in a refining module; this is no longer so.
That is, 'decreases *' is now inherited.  To refine a possibly non-terminating method
or loop, the refining version simply provides a decreases clause that does not mention '*'.
Note that if the refined method is not recursive, it still needs to have _some_ decreases
clause in order not to inherit the 'decreases *' from the refined method, but the expression
stated in the decreases clause can be arbitrary (for example, one can write 'decreases true'
or 'decreases 7' or 'decreases x' for some 'x' in scope).

Note, in the new design, a method needs to be declared with 'decreases *' if
it may recurse forever _or_ if it contains a possibly infinite loop.

Note that the absence of 'decreases *' on a loop does not mean the loop will
terminate, but it does mean that the loop will iterate a finite number of times
(the subtle distinction here is that a loop without a 'decreases *' is allowed
to contain a nested loop that has a 'decreases *' -- provided the enclosing
method is also declared with 'decreases *', as previously mentioned).

Source/Dafny/DafnyAst.cs
@@ -1816,6 +1816,7 @@ namespace Microsoft.Dafny {
     ModuleDefinition EnclosingModule { get; }  // to be called only after signature-resolution is complete
     bool MustReverify { get; }
     string FullSanitizedName { get; }
+    bool AllowsNontermination { get; }
   }
   /// <summary>
   /// An ICallable is a Function, Method, or IteratorDecl.
@@ -1858,6 +1859,7 @@ namespace Microsoft.Dafny {
     ModuleDefinition ICodeContext.EnclosingModule { get { return Module; } }
     bool ICodeContext.MustReverify { get { Contract.Assume(false, "should not be called on NoContext"); throw new cce.UnreachableException(); } }
     public string FullSanitizedName { get { Contract.Assume(false, "should not be called on NoContext"); throw new cce.UnreachableException(); } }
+    public bool AllowsNontermination { get { Contract.Assume(false, "should not be called on NoContext"); throw new cce.UnreachableException(); } }
   }
 
   public class IteratorDecl : ClassDecl, IMethodCodeContext
@@ -1959,6 +1961,11 @@ namespace Microsoft.Dafny {
     }
     ModuleDefinition ICodeContext.EnclosingModule { get { return this.Module; } }
     bool ICodeContext.MustReverify { get { return false; } }
+    public bool AllowsNontermination {
+      get {
+        return Contract.Exists(Decreases.Expressions, e => e is WildcardExpr);
+      }
+    }
   }
 
   public abstract class MemberDecl : Declaration {
@@ -2451,6 +2458,12 @@ namespace Microsoft.Dafny {
       }
     }
 
+    public bool AllowsNontermination {
+      get {
+        return Contract.Exists(Decreases.Expressions, e => e is WildcardExpr);
+      }
+    }
+
     /// <summary>
     /// The "AllCalls" field is used for non-CoPredicate, non-PrefixPredicate functions only (so its value should not be relied upon for CoPredicate and PrefixPredicate functions).
     /// It records all function calls made by the Function, including calls made in the body as well as in the specification.
@@ -2683,6 +2696,11 @@ namespace Microsoft.Dafny {
       }
     }
     bool ICodeContext.MustReverify { get { return this.MustReverify; } }
+    public bool AllowsNontermination {
+      get {
+        return Contract.Exists(Decreases.Expressions, e => e is WildcardExpr);
+      }
+    }
   }
 
   public class Lemma : Method
